
---
excalidraw-default-mode: view
---

```toc

```

^TOC

<[[2022-2023 Sophomore/Winter Quarter/ECE205-04_Circuits_and_Systems/2022-11-28|previous]] | [[2022-12-02|next]]>

## Lecture 2

### Previous class:

$$\tau\cdot\dot{y}(t) + y(t) = k\cdot x(t)$$

### Example 2

![[Drawing 2022-11-29 09.02.50.excalidraw|10000]]

$$\frac{V_s(t)-V_l(t)}{R_a}=i_L(t)+\frac{V_L(t)}{R_0}$$
$$(\frac{R_a+R_0}{R_aR_0})L\frac{di_L(t)}{dt}+i_L(t) = \frac{1}{R_a}V_s(t)$$
$$\tau=(\frac{R_a+R_0}{R_aR_0})L$$
$$k=\frac{1}{R_a}$$


### Example 3

![[Drawing 2022-11-29 09.09.38.excalidraw|10000]]
$$\frac{V_s(t)-V_C(t)}{R_a}=C\frac{dV_C(t)}{dt}+\frac{V_C(t)}{R_b}$$
$$(\frac{R_aR_b}{R_a+R_b})C\frac{dV_C(t)}{dt} +V_C(t)=\frac{R_b}{R_a+R_b}V_s(t)$$
$$\tau = (\frac{R_aR_b}{R_a+R_b})$$
$$k = \frac{R_b}{R_a+R_b}$$


### Example 4 in OneNote

### Shortcut for FIRST ORDER ONLY

<u>Thevenin resistance, time constants, static gain</u>

For out first order circuits, we can derive/check our constants using the following relationships:

1. $\tau = R_{TH}\cdot C_{eq},\; \tau=\frac{L_{eq}}{R_{TH}}$ Where $R_{TH}$ is the equivalent resistance as seen from the ports of the L or C.
2. In steady state, with a DC source, (with a stepped DC input) $y(\infty) = k\cdot x(\infty)$ where $y$ and $x$ are the values at the source.
	1. C = open
	2. L = short

Regardless of the actual input, we can assume that input is a stepped DC input in order to find $k$.



### Solving First Order LTI Differential Equations

There are two common methods:
1. D solution = natural response + forced response
2. Integrating factors

#### Method 1
Solve: 
$$\tau\cdot\dot{y}+y(t) = Kx(t)$$
$y(t)$ is the natural response, which is the response with no inputs. $(x(t)=0)$
$y(f(t))$ is the forced response, (response due to input $x(t)$)

**Natural response:**
$$\tau\cdot\dot{y}_n(t)+y_n(t)=0$$

> Assume: $y_n(t) = ce^{rt},\;\dot{y}_n=cre^{rt}$

$$\tau(cre^{rt}+ce^{rt}) = 0$$
$$ce^{rt}(\tau r + 1) = 0$$
> $ce^{rt}$ will never be zero, so we can ignore it

$$\tau r + 1 = 0$$
$$r= \frac{-1}{\tau}$$

> now $y_n(t)=ce^{\frac{-t}{\tau}}$



