---
excalidraw-default-mode: view
---


```toc

```

^TOC

<[[2022-2023 Sophomore/MA276 Intro To Proofs/Notes/2022-09-13|previous]] | [[|next]]>

### Example continuing from previous

Proof: Suppose x and y are integers such that x and y are both off. This means that $\exists k,j \in \mathbb{Z}$ such that $x=2k+1$ and $y=2j+1$. Then $x+y=(2k+1)+(2j+1) = 2k + 2j + 2 = 2(k+j+1)$. Let $n = k+j+1$. Note $n \in \mathbb{Z}$ Since $x+y = 2n$ so $x+y$ is even. $\blacksquare$

#### Note:
When writing a proof in paragraph form, $\exists k,j \in \mathbb{Z}$ such that $x=2k+1$ and $y=2j+1$. this defines k,j,x,y for the entirety of the proof, unlike in a purely symbolic proof where the there exists needs to follow k,j for every equivalence.


## Indirect proof example:
Suppose $n$ is an integer. If $n^2$ is not even, then n is not even.

> Instead of proving this statement, we are going to prove the contrapositive

If $n$ is even, then $n^2$ is even

---
------ SCRATCH ------

|<u>Givens</u>|<u>Goals</u>|
| :---: | :---: |
|$n\in\mathbb{Z}$| $n^2 = 2j$ for some $k \in \mathbb{Z}$|
|$n=2k$ for some $k \in \mathbb{Z}$ | |

----- End Scratch ------


---

<u>Proof:</u> Suppose n is an integer. We aim to prove the contrapositive of if $n^2$ is not even, then n is not even. Toward that end, assume n is even. This means that $\exists k \in\mathbb{Z}$ such that $n=2k$.

Then, $n^2 = (2k)^2 = 4k^2 = 2(2k^2)$
Let $j=2k^2$, so $n^2 = 2j$.
Since $j\in\mathbb{Z}$, we know that n is even. $\quad\blacksquare$


### More example:

Suppose $A\cap B \subseteq C\backslash D$
If $x\in A$, then if $x\in D$ then $x \notin B$


---
------ SCRATCH ------


|<u>Givens</u>|<u>Goals</u>|
| :---: | :---: |
|$A \cap B \subseteq C \backslash D$  | $x\in A \to [x \in D \to x \notin B]$ |

Direct Proof:

|<u>Givens</u>|<u>Goals</u>|
| :---: | :---: |
|  $A \cap B \subseteq C \backslash D$ | $x \in D \to x \notin B$|
| $x \in A$ |  |


Indirect Proof:


|<u>Givens</u>|<u>Goals</u>|
| :---: | :---: |
| $A \cap B \subseteq C \backslash D$ | $x \in D$ |
| $x \in A$ |  |
| $x \in B$ |  |

----- End Scratch ------

---

<u>proof:</u> Suppose $A \cap B \subseteq C \backslash D$ and $x \in A$. We aim to prove the contrapositive of $x \in D \to x \notin B$. Towards that end, we are going to suppose that $x \in B$. Since $x \in A$ and $x\in B$, we know that x is in the intersection of those two sets: $x \in A\cap B$. Since our intersection is a subset of $C\backslash D$, we know that also $x \in C\backslash D$. This means that $x \in C \land x \notin D$. This means that $x\in C$, but more importantly, $x \notin D$. $\quad\blacksquare$


## Third Strategy - Proof by Contradiction

>Assume P is true, and show that this leads to something absurd.


|<u>Givens</u>|<u>Goals</u>|
| :---: | :---: |
|$P$|$\neg P$|

### Example
Suppose $\neg R \to (P \to \neg Q)$ is true.
Then $P \to (Q \to R)$ is true.


---
------ SCRATCH ------

|<u>Givens</u>|<u>Goals</u>|
| :---: | :---: |
|$\neg R \to (P \to \neg Q)$|$Q \to R$|
|$P$||

$\downarrow$

|<u>Givens</u>|<u>Goals</u>|
| :---: | :---: |
|$\neg R \to (P \to \neg Q)$|$R$|
|$P$||
|$Q$||

$\downarrow$

Use a Proof by contradiction:

|<u>Givens</u>|<u>Goals</u>|
| :---: | :---: |
|$\neg R \to (P \to \neg Q)$|$\text{false}$|
|$P$||
|$Q$||
|$\neg  R$||

----- End Scratch ------

---

<u>Proof:</u> Suppose $\neg R \to (P \to \neg Q)$ is true and suppose $P$ is true. We want to show $Q \to R$, so suppose $Q$ is true. Now we want to show that $R$ is true.
