---
excalidraw-default-mode: view
---


```toc

```

^TOC

<[[2022-2023 Sophomore/MA276 Intro To Proofs/Notes/2022-09-08|previous]] | [[|next]]>


## Continuing from last class

### Example Translations:
a. The sum of two non-zero integer squares is sometimes an integer squared.

$$\exists x,y,z \in \mathbb{Z^+} \cup \mathbb{Z^-} [x^2 + y^2 = z^2]$$
The $\exists$ is the translation for ***sometimes***.

b. If $A \cap B = \emptyset,\;\text{then} B\backslash A = B$

$$\neg \exists x (x \in A\land x \in B) \to \forall x ((x\in B \land \neg ( x \in A)) \leftrightarrow (x\in B)) $$

**Non-Zero Integers:**
$$\mathbb{Z^+}\cup\mathbb{Z^-}$$
$$\mathbb{Z}\backslash\{0\}$$

## Quantifier Negation Laws

$$\neg \exists x P(x) \equiv \forall x \neg P(x)$$
$$\text{There does not exist and x, so that P(x) is true}$$
$$\text{is equivalent to:}$$
$$\text{For all x, not P(x) is true.}$$
$$ $$

$$\neg \forall x P(x) \equiv \exists x \neg P(x)$$

<u>Note:</u>
Combining these laws with DeMorgan's Law and other logical equivalences, we are often able to:
(a) build more complex logical equivalences 
(b) Reframe a negative statements as equivalent positive statements

<u>Other Rules:</u>
- Two existential quantifiers in a row $\exists x \exists y$ can be switched without changing the meaning. The previous statement reads: "There exists an x and y such that...". That is equivalent to $\exists y \exists x$, and if x and y are in the same universe of discourse, they can be lumped into $\exists x,y$
- Two universal quantifiers in a row have that the same 

### Example:
show that the statements $A\subseteq B$ and $A\cup B = B$ are logically equivalent.

We have two starting points:
$$A\subseteq B \quad \forall x(x\in A \to x \in B)$$
$$A\cup B = B: \forall x ( x \in A \lor x \in B \$$


Start with the second because it's easier to manipulate.

$$\forall x ( x\ in A \lor x \in B \leftrightarrow x \in B)$$
$$\equiv \forall x ((( x \in A \lor x \in B) \to x \in B) \land ( x \in B \to x \in A \lor x \in B))$$

$$( x \in B \to x \in A \lor x \in B)) \;\text{is a tautology}$$
$$\therefore\; \forall x ((( x \in A \lor x \in B) \to x \in B)$$
$$\forall x ((x \in A \to x \in B) \land (x \in B \to x \in B)$$
$$x \in B \to x \in B)\;\text{is a tautology}$$
$$\therefore \forall x ( x \in A \to x \in B)$$
