---
excalidraw-default-mode: view
---


```toc

```

^TOC

<[[2022-2023 Sophomore/MA276 Intro To Proofs/Notes/2022-10-25|previous]] | [[|next]]>

## Defining Recursively defined things

<u>definition:</u> Let $A$ be a set and let $f:\mathbb{Z}^+\to A$ and let $g:A\to A$.
> Note: A can not be empty because $f$ is a function, and therefore $A$ must have at least one element.

Suppose $f$ can be defined as follows:
$$f(1) = a_0$$
$$f(n+1) = g(f(n)) \;\text{for}\;n\geq 1$$

We saw $f$ is defined recursively or is a recursive function.


### Example

1. Let $g:\mathbb{Z}\to\mathbb{Z}, g(x) = 2x$
	Let $f:\mathbb{Z}^+\to \mathbb{Z}. f(1) = 2, f(n+1) = g(f(n))$
	This is the recursive definition  = $h(n) = 2^n$

> We use the more complicated recursive definitions in order to be able to prove facts about them using induction.

2. $g:\mathbb{Z}\to\mathbb{Z}$ and $f:\mathbb{Z}^+\to\mathbb{Z}$ be defined as
$$f(1) = g(1)$$
$$f(n+1) = f(n)+g(n+1)$$

So this is recursive definition of $$h(n) = \sum_{k=1}^ng(k)$$.


### Example Fibonacci
Let $g: \mathbb{Z}\times\mathbb{Z} \to \mathbb{Z}$ be defined by $g(x,y) = x+y.$ 
Let $f:\mathbb{Z}\to\mathbb{Z}^+$ be defined:
$$f(1) = 1$$
$$f(2) = 1$$
$$f(n+1) = g(f(n),f(n-1))$$

###