---
excalidraw-default-mode: view
---


```toc

```

^TOC

<[[2022-2023 Sophomore/MA276 Intro To Proofs/Notes/2022-09-15|previous]] | [[|next]]>


### Example from yesterday contd. 
Suppose $\neg R \to (P \to \neg Q)$ is true.
Then $P \to (Q \to R)$ is true.


---
------ SCRATCH ------

|<u>Givens</u>|<u>Goals</u>|
| :---: | :---: |
|$\neg R \to (P \to \neg Q)$|$Q \to R$|
|$P$||

$\downarrow$

|<u>Givens</u>|<u>Goals</u>|
| :---: | :---: |
|$\neg R \to (P \to \neg Q)$|$R$|
|$P$||
|$Q$||

$\downarrow$

Use a Proof by contradiction:

|<u>Givens</u>|<u>Goals</u>|
| :---: | :---: |
|$\neg R \to (P \to \neg Q)$|$\text{false}$|
|$P$||
|$Q$||
|$\neg  R$||

----- End Scratch ------

---

<u>Proof:</u> Suppose $\neg R \to (P \to \neg Q)$ is true and suppose $P$ is true. We want to show $Q \to R$, so suppose $Q$ is true. Now we want to show that $R$ is true.

Suppose by way of contradiction that $\neg R$ is actually true. Since $\neg R$ and $\neg R \to (P \to \neg Q)$ is true, $P \to \neg Q$ is true.
