---
excalidraw-default-mode: view
---


```toc

```

^TOC

<[[2022-2023 Sophomore/MA276 Intro To Proofs/Notes/2022-11-01|previous]] | [[|next]]>

### Theorem

 Let $a,b \in \mathbb{Z}^+$ such that $b\nmid a.$ Suppose the Divisional Algorithm produces $q$ and $r$ such that $a = qb+r$ and $0<r<b.$ Then $\text{gcd}(a,b)=\text{gcd}(r,b).$

<u>proof</u>: To show $\text{gcd}(a,b)=\text{gcd}(r,b)$ we will show $\text{gcd}(a,b)\mid\text{gcd}(r,b)$ AND $\text{gcd}(r,b)\mid\text{gcd}(a,b)$

Note: $a = qb + r.$

We know $\text{gcd}(r,b)\mid r$ and $\text{gcd}(r,b)\mid qb$