---
excalidraw-default-mode: view
---


```toc

```

^TOC

<[[2022-2023 Sophomore/MA276 Intro To Proofs/Notes/2022-10-11|previous]] | [[[|next]]>

> Finished the previous in class example in the previous note.

### Example

Let $A = \mathbb{R}\backslash \{2\}$ and $B = \mathbb{R}\backslash \{3\}$. Prove that $f:A\to B$ defined by $x\rightarrowtail \frac{3x}{x-2}$ is invertible (meaning that $f^{-1}$ is a function) and find $f^{-1}$. 

> To prove that $f^{-1}$ is a function, we can use the previously described theorem by showing that $f$ is bijective, which implies that $f^{-1}$ is a function.


<u>proof</u>. (INJECTIVE) Let $x,y \in A$ such that $f(x) = f(y)$. We want to show $x=y$. Then 
$$\frac{3x}{x-2} = \frac{3y}{y-2}$$
$$3xy-6x=3xy-6y$$
$$-6x=-6y$$
$$x=y$$
So $f$ is injective.

(SURJECTIVE) Let $z \in B$.

---
--- SCRATCH ---
$$\frac{3x}{x-2} = z$$
$$3x=xz-2z$$
$$x(3-z) = -2z$$
$$x = \frac{2z}{z-3}$$

--- END SCRATCH ---

--- 

Set $x := \frac{2z}{z-3}$. Note $x$ is defined because $z\neq 3$, so $x \in \mathbb{R}$. Suppose $x=2$. Then $2=\frac{2x}{z-3}\to 2z-6=2z \to-6=0$, a contradiction. So $x \neq 2$, and $x\in \mathbb{R}\backslash\{2\}$.

Consider $f(x)$. 

$$f(x) = \frac{3(\frac{2z}{z-3})}{(\frac{2z}{z-3})-2}$$
$$= \frac{6z}{2z-2(z-3)}$$
$$= \frac{6z}{6}$$
$$= z\quad\blacksquare$$

Therefore $f$ is surjective and $f^{-1}$ is a function, AND $f^{-1}(z) = \frac{2z}{z-3}$.

## Theorem

Let $A$ and $B$ be non-empty sets and let $f:A\to B$. then $f^{-1}$ is a function if and only if $f\circ f^{-1} = \iota_B$ and $f^{-1}\circ f =\iota_A$.
> $\iota_A$ is the identity relation where every element is mapped only to itself.

<u>proof</u>. $(\to)$ Suppose $f^{-1}$ is a function. We want to show $f^{-1}\circ f = \iota_A$. (We will do this by showing $f^{-1}\circ f \subseteq \iota_A$ and $\iota_A \subseteq f^{-1}\circ f$).
Let $a_1,a_2 \in A$ such that $(a_1,a_2)\in f^{-1}\circ f$. Then $\exists b \in B$ such that $(a_1,b) \in f$ and $(b_,a_2) \in f^{-1}$. Then $(b_1,a_1) \in f^{-1}$. Since $f^-1$ is a function, $a_1 = a_2$. Since $a_1 = a_2, (a_1,a_2)\in \iota_A.$T