---
excalidraw-default-mode: view
---


```toc

```

^TOC

<[[2022-2023 Sophomore/MA276 Intro To Proofs/Notes/2022-09-09|previous]] | [[|next]]>

### Example 2 Continued:
Show the statements $C \subseteq (A\cup B)$ and $(C\backslash A) \subseteq B$ are logically equivalent.

Two starting points:
$$\forall x (x\in C \to (x \in A \lor x \in B))$$
$$\forall x (x \in C \land \neg (x\in A) \to x \in B)$$

proof:
$$\forall x (x \in C \land \neg (x\in A) \to x \in B)$$
is equivalent to
$$\forall (\neg (x \in C \land \neg (x\in A))\lor x \in B)$$
is equivalent
$$\forall x ((\neg(x\in V)\lor(x\in A)\lor x \in B))$$
$$\forall x (\neg ( x\in C) \lor (x \in A \lor x \in B))$$
is equivalent to
$$\forall x ( x\in C \to x \in A \lor x \in B) \quad\blacksquare$$


## On Sets

Current Way:
$$\{ x \in \mathbb{z} : \exists y \in \mathbb{Z} [y^3=x]\}$$
This above way goes universe to predicate.
Instead we can:
$$\{y^3 : y\in\mathbb{Z}\}$$
go from expression to indexset

Index sets can be anything. In the abstract, we use I to denote the indexing set.

$$\{x \in \mathcal{U}:\exists I \in I [x=a_i]\} = \{a_i : i \in I\}$$
where $$



