---
excalidraw-default-mode: view
---


```toc

```

^TOC

<[[2022-2023 Sophomore/MA276 Intro To Proofs/Notes/2022-09-12|previous]] | [[|next]]>


### Example:
![[Drawing 2022-09-13 11.05.42.excalidraw|1000)]]


### Theorem:

Let $\mathcal{R},\mathcal{S}$ be families of subsets in a universe $\mathcal{U}$. Then $[\bigcap\mathcal{R}] \cap [\bigcap \mathcal{S}] = \bigcap[\mathcal{R}\cap \mathcal{S}]$

Proof:

Let $x \in \mathcal{U}$ then $x\in[\bigcap R]\cap[\bigcap{S}] \equiv x\in \bigcap \mathcal{R} \land x \in \bigcap \mathcal{S}$
$$\equiv [\forall X \in \mathcal{R}[x\in X]]\land[\forall X \in \mathcal{S}[x\in X]]$$
$$\equiv [\forall X \in \mathcal{P}(\mathcal(U))[X \in \mathcal{R} \to x \in X]]\land [\forall X ]\in \mathcal{P}(\mathcal{U})[X\in\mathcal{S}\to x \in X]]$$
$$\text{expanding the scope}$$
$$\equiv \forall X \in \mathcal{P}(\mathcal{U})[(X\in\mathcal{R} \to x \in X)\land(X \in \mathcal{S}\to x \in X)]$$
$$\equiv \forall X \in \mathcal{P}(\mathcal{U})[(X \notin \mathcal{R}\lor x \in X)\land (X \notin \mathcal{S} \lor x \in X)]$$
$$\equiv \forall X \in \mathcal{P}(\mathcal{U})[(X \notin R \land X \notin \mathcal{S})\lor x\in X]$$
$$\equiv \forall X \in \mathcal{P}(\mathcal{U})[\neg(X \in \mathcal{R}\lor X \in \mathcal{S})\lor x \in X]$$
$$\equiv \forall X \in \mathcal{P}(\mathcal{U})[(X \in \mathcal{R}\lor X \in \mathcal{S})\to x \in X]$$
$$\equiv \forall X \in \mathcal{P}(\mathcal{U})[(X \in \mathcal{R}\cup \mathcal{S})\to x \in X]$$
$$\text{(Now we want to restrict the scope of the statement)}$$
$$\equiv \forall X \in \mathcal{R}\cup \mathcal{S}[x \in X]$$
$$\equiv x \in \bigcap(\mathcal{R} \cup \mathcal{S}) \;\blacksquare$$

## Chapter 3 - Proof Strategies
The most basic statement we'll consider is the $P \to Q$.

There are two strategies we'll develop to handle this.

1. Direct proof.
		We assume P, and then show that Q follows from that assumption.

2. Indirect proof.
		Recall that $P\to Q \equiv \neg Q \to \neg P$ (contrapositive) In an indirect proof, we assume $\neg Q$ and show that $\neg P$ must follow.

### Example
Suppose x and y are integers. If x and y are odd, then x + y is even.
\-\-\-\-\-\-\-START WITH SCRATCH WORK \-\-\-\-\-\-\-\-

| Givens | Goals |
| :---: | :---: |
|$x,y\in\mathbb{Z}$|x + y is even |
|x is odd | |
|y is odd | |

$\downarrow$

| Givens | Goals |
| :---: | :---: |
|$x,y\in\mathbb{Z}$|$x+y = 2n$ for some $x\in \mathbb{Z}$|
|$x \in 2k+1$ for some $k\in\mathbb{Z}$ | |
|$y \in 2j+1$ for some $j\in\mathbb{Z}$ | |

\-\-\-\-\-\-\-END SCRATCH WORK \-\-\-\-\-\-\-\-





